src/rocq/Utils/NoSpecEvent.v
@@ -1,0 +1,515 @@
+(* begin hide *)
+From Stdlib Require Import
+     RelationClasses
+     Morphisms
+     Program.Equality.
+
+From Paco Require Import paco.
+From ITree Require Import
+     ITree
+     ITreeFacts
+     Eq.Eqit.
+
+From ITreeSpec Require Import
+  ITreeSpecDefinition
+  ITreeSpecFacts
+  ITreeSpecCombinatorFacts.
+
+Set Implicit Arguments.
+Set Strict Implicit.
+(* end hide *)
+
+(** * NoEvent
+    We develop in this file a theory to reason about absence of a given event signature
+    in a tree, and how to use this absence to safely eliminate this signature from the tree.
+ *)
+
+(** * Signature vacuousness
+  A simple way to assert the absence of a signature is based on the shape of the signature.
+  We define straightforward non-recursive functors and take the cofixed points.
+ *)
+
+(* The left part of the signature is absent *)
+Variant no_spec_event_F {E X} (R: itree (SpecEvent E) X -> Prop) : itree' (SpecEvent E) X -> Prop :=
+| no_spec_event_ret: forall (x: X), no_spec_event_F R (RetF x)
+| no_spec_event_tau: forall t, R t -> no_spec_event_F R (TauF t)
+| no_spec_event_vis: forall {Y} (e: E Y) k, (forall x, R (k x)) -> no_spec_event_F R (VisF (Spec_vis e) k).
+#[export] Hint Constructors no_spec_event_F : core.
+
+Lemma no_spec_event_F_mono : forall {E X} (R1 R2 : itree (SpecEvent E) X -> Prop) (LE : R1 <1= R2),
+    no_spec_event_F R1 <1= no_spec_event_F R2.
+Proof using.
+  intros.
+  induction PR; auto.
+Qed.
+
+Definition no_spec_event_F_ {E X} R (t : itree (SpecEvent E) X) := no_spec_event_F R (observe t).
+#[export] Hint Unfold no_spec_event_F_ : core.
+
+Lemma no_event_lF__mono : forall E X, (monotone1 (@no_spec_event_F_ E X)).
+Proof using.
+  do 2 red.
+  intros.
+  eapply no_spec_event_F_mono; eauto.
+Qed.
+
+#[export] Hint Resolve no_spec_event_F_mono : paco.
+
+Definition no_spec_event {E X} := paco1 (@no_spec_event_F_ E X) bot1.
+
+(* This exists in the stdlib as [ProofIrrelevance.inj_pair2], but we reprove
+   it to not depend on proof irrelevance (we use axiom [JMeq.JMeq_eq] instead).
+   The itree library now avoids as much as possible using this axiom, we may want
+   to see if it's possible to do so here.
+ *)
+Lemma inj_pair2 :
+  forall (U : Type) (P : U -> Type) (p : U) (x y : P p),
+    existT P p x = existT P p y -> x = y.
+  Proof using.
+    intros. apply JMeq.JMeq_eq.
+    refine (
+        match H in _ = w return JMeq.JMeq x (projT2 w) with
+        | eq_refl => JMeq.JMeq_refl
+        end).
+  Qed.
+
+(** up-to eq_itree closure
+  Coinductive proofs about no_spec_event can be performed up-to `eq_itree`.
+
+  Note that up-to eutt is not valid:
+    Tau (Vis e k)
+        |  no_spec_eventF
+        v
+      Vis e k ~~ Tau (Vis e k)
+
+  Up-to euttge is valid as well.
+  *)
+Section eqit_closure.
+
+  Inductive eqit_clo {E R} (r : itree E R -> Prop)
+    : itree E R -> Prop :=
+  | eqit_clo_intro b t t' (EQVl: eqit eq b false t t') (REL: r t')
+    : eqit_clo r t.
+  Hint Constructors eqit_clo: core.
+
+  Lemma eqit_clo_mon {E R} r1 r2 t
+        (IN: eqit_clo r1 t)
+        (LE: r1 <1= r2):
+    @eqit_clo E R r2 t.
+  Proof using.
+    destruct IN. econstructor; eauto.
+  Qed.
+
+  Lemma no_spec_event_eqit_clo_wcompat {E R} :
+    wcompatible1 (@no_spec_event_F_ E R) eqit_clo.
+  Proof using.
+    econstructor.
+    pmonauto.
+    intros.
+    inversion PR.
+    punfold EQVl.
+    unfold_eqit.
+    unfold no_spec_event_F_ in *.
+    induction EQVl; auto.
+    - inversion REL.
+      constructor.
+      pclearbot.
+      gclo; econstructor; cycle -1; eauto with paco.
+    - subst. destruct e.
+      + constructor.
+        dependent induction REL.
+        pclearbot; intros; gclo; econstructor; cycle -1; eauto with paco.
+        apply REL0.
+      + inversion REL.
+      + inversion REL.
+    - constructor.
+      gstep; auto.
+    - congruence.
+  Qed.
+
+  #[global] Instance eq_itree_no_spec_event_l_cong {E R} r rg :
+    Proper ((eq_itree eq) ==> flip impl) (gpaco1 (@no_spec_event_F_ E R) eqit_clo r rg).
+  Proof using.
+    repeat intro.
+    gclo.
+    econstructor; cycle -1; eauto.
+  Qed.
+
+  #[global] Instance euttge_no_spec_event_l_cong {E R} r rg :
+    Proper ((euttge eq) ==> flip impl) (gpaco1 (@no_spec_event_F_ E R) eqit_clo r rg).
+  Proof using.
+    repeat intro.
+    gclo.
+    econstructor; cycle -1; eauto.
+  Qed.
+
+End eqit_closure.
+#[export] Hint Resolve eqit_clo_mon : paco.
+#[export] Hint Constructors eqit_clo: core.
+#[export] Hint Resolve no_spec_event_eqit_clo_wcompat : paco.
+
+(* In particular [eq_itree] is hence a congruence for [no_spec_event] *)
+#[global] Instance no_spec_event_eq_itree {E X} : Proper (eq_itree eq ==> iff) (@no_spec_event E X).
+Proof using.
+  repeat red. intros. split; intros.
+  ginit. rewrite <- H. gfinal; auto.
+  ginit. rewrite H. gfinal; auto.
+Qed.
+
+(* But although not a valid up-to, [eutt] is also a congruence for [no_spec_event] *)
+#[global] Instance no_spec_event_eutt {E X} : Proper (eutt eq ==> iff) (@no_spec_event E X).
+Proof using.
+  do 2 red.
+  repeat red. intros. split; intros.
+  - revert x y H H0.
+    pcofix CIH.
+    intros x y H0 H1.
+    + punfold H0. red in H0.
+      punfold H1. red in H1.
+      genobs x ox.
+      genobs y oy.
+      pstep. red.
+      revert x Heqox y Heqoy.
+      induction H0; inversion H1; intros; subst.
+      * rewrite <- Heqoy. econstructor.
+      * rewrite <- Heqoy. econstructor. pclearbot. right. eapply CIH. 2:  { apply H0. }  apply REL.
+      * rewrite <- Heqoy. destruct e.
+        --  inversion H1. econstructor. intros.
+            specialize (REL x0). red in REL. pclearbot. right. eapply CIH. apply REL.
+            apply inj_pair2 in H3. rewrite <- H3. specialize (H0 x0). apply H0.
+        --  inversion H1.
+        --  inversion H1.
+      * eapply IHeqitF. pclearbot. punfold H2. reflexivity. reflexivity.
+      * rewrite <- Heqoy. econstructor. left.
+        pstep. red. eapply IHeqitF. econstructor. apply Heqox. reflexivity.
+      * rewrite <- Heqoy. econstructor. left.
+        pstep. red. eapply IHeqitF. econstructor. assumption. apply Heqox. reflexivity.
+      * rewrite <- Heqoy. econstructor. left.
+        pstep. red. eapply IHeqitF. econstructor. intros. apply H. apply Heqox. reflexivity.
+  - revert x y H H0.
+    pcofix CIH.
+    intros x y H0 H1.
+    + punfold H0. red in H0.
+      punfold H1. red in H1.
+      genobs x ox.
+      genobs y oy.
+      pstep. red.
+      revert x Heqox y Heqoy.
+      induction H0; inversion H1; intros; subst.
+      * rewrite <- Heqox. econstructor.
+      * rewrite <- Heqox. econstructor. pclearbot. right. eapply CIH. 2:  { apply H0. }  apply REL.
+      * rewrite <- Heqox. destruct e. inversion H1. econstructor. intros.
+        -- specialize (REL x0). red in REL. pclearbot. right. eapply CIH. apply REL.
+           apply inj_pair2 in H3. rewrite <- H3. specialize (H0 x0). apply H0.
+        -- inv H1.
+        -- inv H1.
+      * rewrite <- Heqox. econstructor. left.
+        pstep. red. eapply IHeqitF. econstructor. reflexivity. apply Heqoy.
+      * rewrite <- Heqox. econstructor. left.
+        pstep. red. eapply IHeqitF. econstructor. assumption. reflexivity. apply Heqoy.
+      * rewrite <- Heqox. econstructor. left.
+        pstep. red. eapply IHeqitF. econstructor. intros. apply H. reflexivity. apply Heqoy.
+      * eapply IHeqitF. pclearbot. punfold H2. reflexivity. reflexivity.
+Qed.
+
+Lemma no_spec_event_to_itree_spec {E X} : forall (t: itree (SpecEvent E) X), no_spec_event (to_itree_spec t).
+Proof using.
+  intros t.
+  setoid_rewrite (itree_eta t).
+  genobs t ot. clear t Heqot.
+  revert ot.
+  pcofix CIH.
+  intros ot.
+  destruct ot; auto.
+  - pstep; red; cbn.
+    constructor.
+  - pstep; red; cbn.
+    constructor.
+    right.
+    unfold to_itree_spec in *.
+    rewrite (EqAxiom.itree_eta_ t).
+    apply CIH.
+  - pstep; red; cbn.
+    constructor.
+    intros x.
+    right.
+    rewrite (EqAxiom.itree_eta_ (k x)).
+    apply CIH.
+Qed.
+
+(** * Signature elimination
+  In order to eliminate a signature from the type,
+  we need to handle it into an itree over the remaining signature.
+  Since the intent is to run these handlers over trees that do not
+  contain such events, how we handle them should not matter, but
+  the obvious solution is to interpret them into [spin]
+ *)
+
+Definition helim_spec {E}: SpecEvent E ~> itree E :=
+  fun _ e => match e with
+          | Spec_vis e => trigger e
+          | Spec_forall _
+          | Spec_exists _ => ITree.spin
+          end.
+
+Definition elim_spec {E}: itree (SpecEvent E) ~> itree E := interp helim_spec.
+
+(** * Soundness
+    The tricky part is now to figure out how to express the correctness of
+    the elimination of vacuous signatures.
+ *)
+
+(** By asserting that handlers can't be distinguished: *)
+
+(* Lemma no_spec_event_elim : *)
+(*   forall {E X} (t : itree (SpecEvent E) X), *)
+(*     no_spec_event t -> *)
+(*     forall (h : E ~> itree E) , elim_spec t  ≈ interp (to_itree_spec_handler h) t. *)
+(* Proof using. *)
+(*   intros E F X. *)
+(*   unfold elim_l. *)
+(*   intros t H h. *)
+(*   revert t H. *)
+(*   einit. *)
+(*   ecofix CIH. *)
+(*   intros. *)
+(*   rewrite (itree_eta t). *)
+(*   pinversion H0. *)
+(*   - rewrite interp_ret. rewrite interp_ret. reflexivity. *)
+(*   - rewrite interp_tau. rewrite interp_tau. estep. *)
+(*   - rewrite interp_vis. rewrite interp_vis. cbn. *)
+(*     unfold id_. unfold Id_Handler, Handler.id_. *)
+(*     ebind. econstructor. reflexivity. *)
+(*     intros. subst. estep. *)
+(*     ebase. right. eapply CIHL. apply H1. *)
+(* Qed. *)
+
+Lemma no_spec_event_interp :
+  forall {E X} (t : itree (SpecEvent E) X),
+    no_spec_event t ->
+    forall (h : E ~> itree E) ,
+      t ≈ interp (to_itree_spec_handler h) t.
+Proof using.
+  intros E X.
+  einit.
+  ecofix CIH.
+  intros t H h.
+  rewrite (itree_eta t).
+  rewrite (itree_eta t) in H.
+  genobs t ot.
+  clear t Heqot.
+  pinversion H; cbn in *; subst.
+  - setoid_rewrite interp_ret. reflexivity.
+  - setoid_rewrite interp_tau. estep.
+  - setoid_rewrite interp_vis. cbn.
+    unfold to_itree_spec.
+    red in H.
+    cbn in *.
+Admitted.
+
+(** By expressing that [elim] is an inverse to the signature injection: *)
+
+(* Injection to the left *)
+Definition inject_spec {E}: itree E ~> itree (SpecEvent E) :=
+  translate (@to_SpecEvent _).
+
+(* For some reason the new definition of [ecofix] in itrees loops here.
+  We redefine the old one for now.
+*)
+Require Import Paco.pacotac_internal.
+
+Tactic Notation "ecofix" ident(CIH) "with" ident(gL) ident(gH) :=
+   repeat red;
+   paco_pre2;
+   eapply euttG_cofix;
+   paco_post2 CIH with gL;
+   paco_post2 CIH with gH.
+
+Tactic Notation "ecofix" ident(CIH) := ecofix CIH with gL gH.
+
+Lemma inject_no_spec_event : forall {E X} t,
+  no_spec_event (@inject_spec E X t).
+Proof using.
+  intros E X.
+  ginit; gcofix CIH; intros t.
+  setoid_rewrite unfold_translate.
+  gstep.
+  destruct (observe t); cbn; constructor.
+  - gbase; apply CIH.
+  - intros ?; gbase; apply CIH.
+Qed.
+
+(* [elim_l] is _always_ a left inverse to [inject_l] *)
+Lemma elim_inject_spec :
+  forall {E X} (t : itree E X),
+    elim_spec (@inject_spec E _ t) ≈ t.
+Proof using.
+  einit.
+  ecofix CIH.
+  intros.
+  rewrite (itree_eta t).
+  unfold elim_spec. unfold inject_spec.
+  destruct (observe t).
+  - rewrite translate_ret. rewrite interp_ret.
+    estep.
+  - rewrite translate_tau. rewrite interp_tau.
+    estep.
+  - rewrite translate_vis. rewrite interp_vis. cbn.
+    rewrite bind_trigger. estep.
+    intros.
+    rewrite tau_eutt. ebase.
+Qed.
+
+(* [inject_l] is a left inverse to [elim_l] when considering trees with [no_spec_event_l] *)
+Lemma inject_elim_spec :
+  forall {E X} (t : itree (SpecEvent E) X),
+    no_spec_event t ->
+    inject_spec (elim_spec t) ≈ t.
+Proof using.
+  einit.
+  ecofix CIH.
+  intros.
+  rewrite (itree_eta t).
+  unfold elim_spec in *.
+  unfold inject_spec in *.
+  pinversion H0.
+  - rewrite interp_ret. rewrite translate_ret. estep.
+  - rewrite interp_tau. rewrite translate_tau. estep.
+  - rewrite interp_vis. rewrite translate_bind.  cbn.
+    unfold trigger.  rewrite translate_vis. rewrite bind_vis.
+    estep. intros. rewrite translate_ret. rewrite bind_ret_l.
+    rewrite translate_tau. rewrite tau_eutt. ebase.
+    left. apply CIH0. apply H1.
+Qed.
+
+(** * Establishing [no_spec_event]
+    If two tree are similar after non-trivial injections, they have no events.
+    The following probably needs to be refined.
+ *)
+
+(*  ------------------------------------------------------------------------- *)
+(* TODO: Move these to the itrees library? *)
+
+Lemma translate_ret_inv : forall E F A (h : E ~> F) (t : itree E A) a,
+    translate h t ≅ ret a -> t ≅ ret a.
+Proof using.
+  intros.
+  rewrite (itree_eta t) in *.
+  pinversion H.
+  destruct (observe t); cbn in *; inversion H1. subst. reflexivity.
+  inversion CHECK.
+Qed.
+
+Lemma translate_tau_inv : forall E F A (h : E ~> F) (t : itree E A) u,
+    translate h t ≅ Tau u -> exists u', t ≅ Tau u'.
+Proof using.
+  intros.
+  setoid_rewrite (itree_eta t).
+  rewrite (itree_eta t) in H.
+  pinversion H; try inversion CHECK.
+  destruct (observe t); cbn in *; inversion H1. subst. exists t0. reflexivity.
+Qed.
+
+Lemma translate_tau_vis : forall E F A B (h : E ~> F) (t : itree E B) f k,
+    translate h t ≅ Vis f k -> exists e k', f = @h A e /\ t ≅ Vis e k'.
+Proof using.
+  intros.
+  setoid_rewrite (itree_eta t).
+  rewrite (itree_eta t) in H.
+  pinversion H; try inversion CHECK.
+  apply inj_pair2 in H3.
+  apply inj_pair2 in H4.
+  subst. destruct (observe t). cbn in *. inversion H1. inversion H1. cbn in *.
+  inversion H. cbn in *.
+  apply inj_pair2 in H3.
+  apply inj_pair2 in H4.
+  subst.
+  apply inj_pair2 in H7.
+  apply inj_pair2 in H6. subst.
+  exists e0.
+  exists k2. split; reflexivity.
+Qed.
+(*  ------------------------------------------------------------------------- *)
+
+#[global] Instance Proper_inject_spec {E X} : Proper (eq_itree eq ==> eq_itree eq) (@inject_spec E X).
+Proof using.
+  do 3 red.
+  intros x y EQ.
+  rewrite EQ. reflexivity.
+Qed.
+
+(* TODO: Probably need to move this *)
+Definition to_spec_handler {E F} (h : E ~> F) : SpecEvent E ~> SpecEvent F.
+  intros T X.
+  destruct X.
+  - apply Spec_vis.
+    apply h; auto.
+  - apply Spec_forall.
+  - apply Spec_exists.
+Defined.
+
+Lemma no_spec_event_translate :
+  forall {E F X} (m : E ~> F) (t : itree (SpecEvent E) X), no_spec_event t -> no_spec_event (translate (to_spec_handler m) t).
+Proof using.
+  ginit.
+  intros E F X m t H.
+  rewrite (itree_eta t).
+  revert t H.
+  gcofix CIH.
+  intros * NEV.
+  rewrite itree_eta in NEV.
+  red in NEV.
+  punfold NEV.
+  inversion NEV.
+  - rewrite translate_ret.
+    gstep.
+    constructor.
+  - pclearbot.
+    rewrite translate_tau.
+    gstep.
+    constructor.
+    rewrite (itree_eta t0).
+    gbase.
+    eauto.
+  - pclearbot.
+    rewrite translate_vis.
+    gstep.
+    red. cbn.
+    constructor.
+    intros x.
+    rewrite (itree_eta (k x)).
+    gbase.
+    eapply CIH.
+    apply H0.
+Qed.
+
+(* And while we're at it, injection should not compromise [no_spec_event] *)
+Lemma no_spec_event_inject :
+  forall {E X} (t : itree E X), no_spec_event (@inject_spec E _ t).
+Proof using.
+  ginit.
+  intros *.
+  rewrite (itree_eta t).
+  genobs t ot.
+  clear t Heqot.
+  revert ot.
+  unfold inject_spec.
+  gcofix CIH.
+  intros ot.
+  hinduction ot before E; intros * CIH.
+  - rewrite translate_ret.
+    gstep.
+    constructor.
+  - rewrite translate_tau.
+    rewrite (itree_eta t).
+    gstep.
+    constructor.
+    gbase.
+    eauto.
+  - rewrite translate_vis.
+    gstep; red; cbn; constructor.
+    intros x.
+    rewrite (itree_eta (k x)).
+    gbase.
+    apply CIH.
+Qed.
